theories/typing/lib/rc/rc.v
@@ -1,4 +1,3 @@
-From Coq.QArith Require Import Qcanon.
 From iris.proofmode Require Import tactics.
 From iris.algebra Require Import auth csum frac agree excl numbers.
 From lrust.lang.lib Require Import memcpy.
@@ -175,7 +174,7 @@ Section rc.
       { iExists _, _, _. iFrame "Hpersist".
         iMod (bor_sep with "LFT HX") as "[Hrc Hlft]"; first solve_ndisj.
         iDestruct (frac_bor_lft_incl with "LFT [> Hlft]") as "$".
-        { iApply (bor_fracture with "LFT"); first solve_ndisj. by rewrite Qp_mult_1_r. }
+        { iApply (bor_fracture with "LFT"); first solve_ndisj. by rewrite Qp_mul_1_r. }
         iApply (bor_na with "Hrc"); solve_ndisj. }
       iApply ("Hclose1" with "[]"). by auto.
     - iMod ("Hclose1" with "[]") as "_"; first by auto.
@@ -591,9 +590,8 @@ Section code.
     iMod (own_update with "Hrc●") as "[Hrc● Hrctok2]".
     { apply auth_update_alloc, prod_local_update_1,
       (op_local_update_discrete _ _ (Some (Cinl ((qb/2)%Qp, 1%positive))))=>-[/= Hqa _].
-      split; simpl; last done. apply frac_valid'. rewrite -H comm_L -{2}(Qp_div_2 qb).
-      apply Qcplus_le_mono_l. rewrite -{1}(Qcplus_0_l (_ / _)%Qp).
-      apply Qcplus_le_mono_r, Qp_ge_0. }
+      split; simpl; last done. apply frac_valid'. rewrite /= -H comm_L.
+      by apply Qp_add_le_mono_l, Qp_div_le. }
     rewrite right_id -Some_op -Cinl_op -pair_op. iDestruct "Hνtok" as "[Hνtok1 Hνtok2]".
     iMod ("Hclose3" with "[$Hrctok] Hna") as "[Hα1 Hna]".
     iMod ("Hclose2" with "[Hrc● Hl'1 Hl'2 Hl'† Hνtok2 Hν† $Hna]") as "Hna".
